\subsection{Adjunkte Matrix}
Sei (R,+,$\cdot$,0,1) ein kommutativer Ring mit Eins. Für $A\in M_n(R)$ definieren wir \newline die Adjunkte von A durch $A^*=(\alpha_{ij}^*)_{ij}$ mit

\[
    (\alpha_{ij}^*)_{ij} := (-1)^{i+j}detA_{ji}
\]
für $i,j\in \{1,\dots,n\}$
\subsection{Beispiel Adjunkte}

Sei $A=\begin{pmatrix}
           1&2&2\\0&1&2\\1&2&0
\end{pmatrix}$ \newline
So ist $A^* = \begin{pmatrix}
                  \alpha_{11}&\alpha_{12}&\alpha_{13}\\
                  \alpha_{21}&\alpha_{22}&\alpha_{23}\\
                  \alpha_{31}&\alpha_{32}&\alpha_{33}
\end{pmatrix}= \begin{pmatrix}
                                 -4&-2&-1\\
                                 -4&-2&0\\
                                 2&2&-4
\end{pmatrix}$ \newline mit \newline\newline
$\alpha_{11}=(-1)^{1+1}detA_{11}=det\begin{pmatrix}1&2\\2&0\end{pmatrix}=1\cdot 0 - 2\cdot2=-4$ \newline
$\alpha_{12}=(-1)^{1+2}detA_{21}=det\begin{pmatrix}0&2\\1&0\end{pmatrix}=0\cdot 0 - 2\cdot1=-2$ \newline
$\alpha_{13}=(-1)^{1+3}detA_{31}=det\begin{pmatrix}0&1\\1&2\end{pmatrix}=0\cdot 2 - 1\cdot1=-1$ \newline
$\alpha_{21}=(-1)^{2+1}detA_{12}=det\begin{pmatrix}2&2\\2&0\end{pmatrix}=2\cdot 0 - 2\cdot2=-4$ \newline
$\alpha_{22}=(-1)^{2+2}detA_{22}=det\begin{pmatrix}1&2\\1&0\end{pmatrix}=1\cdot 0 - 2\cdot1=-2$ \newline
$\alpha_{23}=(-1)^{2+3}detA_{32}=det\begin{pmatrix}1&2\\1&2\end{pmatrix}=1\cdot 2 - 2\cdot1=0$ \newline
$\alpha_{31}=(-1)^{3+1}detA_{13}=det\begin{pmatrix}2&2\\1&2\end{pmatrix}=2\cdot 2 - 2\cdot1=2$ \newline
$\alpha_{32}=(-1)^{3+2}detA_{23}=det\begin{pmatrix}1&2\\0&2\end{pmatrix}=1\cdot 2 - 2\cdot0=2$ \newline
$\alpha_{33}=(-1)^{3+3}detA_{33}=det\begin{pmatrix}1&2\\2&0\end{pmatrix}=1\cdot 0 - 2\cdot2=-4$ \newline